Gonna try something

theories/partial/classical.v
@@ -184,6 +184,132 @@ Proof.
   intros.
   unfold propBind, choice.
   simpl.
+Abort.
+
+(* We do need partiality for general recursion. Will this work? *)
+Definition Partial (T : Type) : Type := Classical (option T).
+  
+Inductive Prog (A B : Type) : Type :=
+| Ret : Partial B -> Prog A B
+| Rec : A -> (B -> Prog A B) -> Prog A B (* TODO: The input should be Partial A instead of just A *)
+.
+
+(* For now I'll keep it a little simpler and now have the def include a partial. *)
+Inductive runProgR {A B : Type} (def : A -> Partial (Prog A B)) : Prog A B -> Partial B -> Prop :=
+| retR : forall b, runProgR def (Ret _ _ b) b
+| recR : forall a b res rest defa,
+    def a = Preturn (Some defa)
+    -> runProgR def defa (Preturn (Some b))
+    -> runProgR def (rest b) res
+    -> runProgR def (Rec _ _ a rest) res
+.
+
+Theorem runProgFunction {A B : Type} {def : A -> Partial (Prog A B)} {p : Prog A B} {b1 b2 : Partial B}
+  (rp1 : runProgR def p b1) (rp2 : runProgR def p b2) : b1 = b2.
+Proof.
+  intros.
+  generalize rp2.
+  generalize b2.
+  clear rp2.
+  clear b2.
+  induction rp1.
+  - intros.
+    inversion rp2.
+    subst.
+    reflexivity.
+  - intros.
+    inversion rp2.
+    subst.
+    apply IHrp1_2.
+    rewrite H in H2.
+    apply PreturnInj in H2.
+    subst.
+    inversion H2.
+    subst.
+    specialize (IHrp1_1 _ H3).
+    apply PreturnInj in IHrp1_1.
+    subst.
+    inversion IHrp1_1.
+    subst.
+    assumption.
+Qed.
+
+Definition runProgImpl {A B : Type} (def : A -> Partial (Prog A B)) (p : Prog A B) : Partial B.
+  refine (exist _ (fun b => runProgR def p (Preturn b)) _).
+  intros.
+  (* I don't think that this will be possible. *)
+  assert (eq := runProgFunction H H0).
+  apply PreturnInj.
+  assumption.
+Defined.
+
+Definition runProg {A B : Type} (def : A -> Partial (Prog A B)) (a : A) : Partial B :=
+  Pbind (def a) (fun a' => 
+                   runProgImpl def a').
+
+Theorem runProgDefinitionRet {A B : Type} (def : A -> Partial (Prog A B)) (b : Partial B)
+  : runProgImpl def (Ret _ _ b) = b.
+Proof.
+  destruct b.
+  apply partialEq.
+  apply functional_extensionality.
+  intros b.
+  apply propositional_extensionality.
+  split.
+  - intros.
+    inversion H.
+    reflexivity.
+  - intros.
+    assert (exist _ x e = Preturn b). {
+      apply itIsReturn.
+      assumption.
+    }
+    rewrite H0.
+    apply retR.
+    (* TODO: would this proof be simpler with definition proof irrelevance? *)
+Qed.
+
+Theorem runProgDefinitionRec {A B : Type} {def : A -> Partial (Prog A B)} {a : A} {rest : B -> Prog A B}
+  : runProgImpl def (Rec _ _ a rest) =
+      Pbind (def a) (fun a' =>
+      Pbind (runProgImpl def a') (fun b =>
+          runProgImpl def (rest b))).
+Proof.
+  apply partialEq.
+  apply functional_extensionality.
+  intros b.
+  apply propositional_extensionality.
+  split.
+  - intros.
+    inversion H.
+    subst.
+    exists defa.
+    split.
+    rewrite H2.
+    reflexivity.
+    exists b0.
+    split.
+    apply H3.
+    apply H5.
+  - intros.
+    destruct H.
+    destruct H.
+    destruct H0.
+    destruct H0.
+
+    Check recR.
+    assert (def a = Preturn x). {
+      induction (def a).
+      apply itIsReturn.
+      simpl in H.
+      assumption.
+    }
+    eapply (@recR _ _ _ _ _ _ _ x H2).
+    simpl in H0, H1.
+    apply H0.
+    apply H1.
+Qed.
+
   
 Lemma lemmaThing (A : Type) (P : A -> Prop) (H : exists a, P a)
   : exists (P' : A -> Prop), exists! a, P' a.
